assign 08

assignments/08/P02.v
@@ -9,13 +9,32 @@ Require Export D.
    (this latter part is trickier than you might expect). *)
 
 Definition pup_to_n : com :=
-  GIVEUP.
+  Y ::= (ANum 0) ;;
+    WHILE BNot (BEq (AId X) (ANum 0)) DO
+          (Y ::= (APlus (AId Y) (AId X)) ;;
+           X ::= (AMinus (AId X) (ANum 1)))
+          END.
 
 Example pup_to_2_ceval :
   pup_to_n / (update empty_state X 2) ||
     update (update (update (update (update (update empty_state
       X 2) Y 0) Y 2) X 1) Y 3) X 0.
 Proof.
-  exact GIVEUP.
+   unfold pup_to_n.
+  apply E_Seq with (update (update empty_state X 2) Y 0).
+  apply E_Ass. reflexivity.
+  apply E_WhileLoop with (update (update (update (update empty_state X 2) Y 0) Y 2) X 1).
+  simpl. reflexivity.
+  apply E_Seq with (update (update (update empty_state X 2) Y 0) Y 2).
+  apply E_Ass. simpl. reflexivity.
+  apply E_Ass. reflexivity.
+  apply E_WhileLoop with  (update (update
+           (update (update (update (update empty_state X 2) Y 0) Y 2) X 1) Y
+           3) X 0). 
+  reflexivity.
+  apply E_Seq with (update (update (update (update (update empty_state X 2) Y 0) Y 2) X 1) Y 3).
+  apply E_Ass. reflexivity.
+  apply E_Ass.  reflexivity.
+  apply E_WhileEnd. reflexivity.
 Qed.
 
