assignments/08/P05.v
@@ -7,7 +7,13 @@ Require Export D.
     same as pushing the value of the expression on the stack. *)
 
 Fixpoint s_compile (e : aexp) : list sinstr :=
-  GIVEUP.
+    match e with
+    | ANum n => [SPush n]
+    | AId i => [SLoad i]
+    | APlus a b => (s_compile a) ++ (s_compile b) ++ [SPlus]
+    | AMinus a b => (s_compile a) ++ (s_compile b) ++ [SMinus]
+    | AMult a b => (s_compile a) ++ (s_compile b) ++ [SMult]
+    end.
 
 (** After you've defined [s_compile], prove the following to test
     that it works. *)
@@ -16,7 +22,7 @@ Example s_compile1 :
     s_compile (AMinus (AId X) (AMult (ANum 2) (AId Y)))
   = [SLoad X; SPush 2; SLoad Y; SMult; SMinus].
 Proof.
-  exact GIVEUP.
+  reflexivity.
 Qed.
 
 (** **** Exercise: 3 stars, advanced (stack_compiler_correct)  *)
@@ -31,11 +37,48 @@ Qed.
     Prove the following theorem, stating that the [compile] function
     behaves correctly.  You will need to start by stating a more
     general lemma to get a usable induction hypothesis; the main
-    theorem will then be a simple corollary of this lemma. *)
+    theorem will then be a simple corollary of this lemma. *) 
+Inductive step : state -> list nat -> sinstr -> list nat -> Prop :=
+| step0 : forall st s n, step st s (SPush n) (n::s)
+| step1 : forall st s i, step st s (SLoad i) (st i::s)
+| step2 : forall st s a b, step st (a::b::s) SPlus (b+a::s)
+| step3 : forall st s a b, step st (a::b::s) SMinus (b-a::s)
+| step4 : forall st s a b, step st (a::b::s) SMult (b*a::s).
 
+Inductive steps : state -> list nat -> list sinstr -> list nat -> Prop :=
+| steps0 : forall st s, steps st s [] s
+| steps1 : forall st s1 s2 s3 instr instrs,
+    step st s1 instr s2 -> steps st s2 instrs s3 ->
+    steps st s1 (instr::instrs) s3.
+
+Lemma steps_execute : forall s st stk1 stk2,
+    steps st stk1 s stk2 -> s_execute st stk1 s = stk2.
+Proof.
+  induction 1. reflexivity. 
+  inversion H; subst; simpl; auto.
+Qed.
+
+Lemma steps_app : forall i1 i2 st s0 s1 s2,
+    steps st s0 i1 s1 ->
+    steps st s1 i2 s2 ->
+    steps st s0 (i1 ++ i2) s2.
+Proof.
+  induction i1; simpl; intros.
+  inversion H; subst; auto.
+  inversion H; subst; auto.
+  inversion H5; subst; econstructor; try constructor; eapply IHi1; eassumption.
+Qed.
+
+Lemma s_compile_steps : forall st e init,
+    steps st init (s_compile e) ( aeval st e :: init ).
+Proof.
+  induction e; simpl; intros; repeat econstructor;
+  repeat (eapply steps_app; try apply IHe1; try apply IHe2); repeat econstructor.
+Qed.
+  
 Theorem s_compile_correct : forall (st : state) (e : aexp),
   s_execute st [] (s_compile e) = [ aeval st e ].
 Proof.
-  exact GIVEUP.
+  intros. apply steps_execute. apply s_compile_steps.
 Qed.
-
+   
