assignments/08/P04.v
@@ -13,6 +13,23 @@ Theorem no_whiles_terminate: forall c st
     (NOWHL: no_whiles c = true),
   exists st', c / st || st'.
 Proof.
-  exact GIVEUP.
+  intros. generalize dependent st. 
+  induction c; intros.
+  exists st. constructor.
+  simpl in *. exists (update st i (aeval st a)). constructor. reflexivity.
+  
+  simpl in *. apply andb_true_iff in NOWHL. inversion NOWHL.
+  apply IHc1 with st in H. inversion H. apply IHc2 with x in H0. inversion H0 as [st2].
+  exists st2.  apply E_Seq with x. apply H1. apply H2. 
+
+  simpl in *. apply andb_true_iff in NOWHL. inversion NOWHL.
+  apply IHc1 with st in H. inversion H.
+  apply IHc2 with st in H0. inversion H0.
+  destruct (beval st b) eqn:B. exists x. apply E_IfTrue. apply B.
+  apply H1. exists x0.  apply E_IfFalse. apply B. apply H2. 
+  inversion NOWHL.  
+
+
+
 Qed.
 
