assignments/08/P07.v
@@ -9,6 +9,13 @@ Theorem IFB_false: forall b c1 c2,
     (IFB b THEN c1 ELSE c2 FI) 
     c2.
 Proof.
-  exact GIVEUP.
+   intros.
+  split. intros.
+  inversion H0; subst.
+  unfold bequiv in H. simpl in H. rewrite H in H6. inversion H6.
+  apply H7.
+  intros. apply E_IfFalse. unfold bequiv in H. simpl in H. rewrite H.
+  reflexivity.
+  apply H0. 
 Qed.
 
