assignments/08/P08.v
@@ -11,6 +11,14 @@ Theorem swap_if_branches: forall b e1 e2,
     (IFB b THEN e1 ELSE e2 FI)
     (IFB BNot b THEN e2 ELSE e1 FI).
 Proof.
-  exact GIVEUP.
+    intros. split; intros.
+  inversion H; subst.
+  apply E_IfFalse. simpl. rewrite H5. reflexivity. apply H6.
+  apply E_IfTrue. simpl. rewrite H5. reflexivity. apply H6.
+  inversion H; subst.
+  apply E_IfFalse. simpl in H5. SearchAbout negb. apply negb_true_iff in H5.
+  apply H5. apply H6.
+  apply E_IfTrue. simpl in H5. apply negb_false_iff in H5. apply H5.
+apply H6. 
 Qed.
 
