assignments/08/P09.v
@@ -5,6 +5,27 @@ Require Export D.
 (** **** Exercise: 2 stars (WHILE_true)  *)
 (** Prove the following theorem. _Hint_: You'll want to use
     [WHILE_true_nonterm] here. *)
+Lemma WHILE_true_nonterm : forall b c st st',
+     bequiv b BTrue ->
+     ~( (WHILE b DO c END) / st || st' ).
+Proof. 
+  (* WORKED IN CLASS *)
+  intros b c st st' Hb.
+  intros H.
+  remember (WHILE b DO c END) as cw eqn:Heqcw.
+  ceval_cases (induction H) Case;
+    (* Most rules don't apply, and we can rule them out 
+       by inversion *)
+    inversion Heqcw; subst; clear Heqcw.
+  (* The two interesting cases are the ones for WHILE loops: *)
+  Case "E_WhileEnd". (* contradictory -- b is always true! *)
+    unfold bequiv in Hb.
+    (* [rewrite] is able to instantiate the quantifier in [st] *)
+    rewrite Hb in H. inversion H.
+  Case "E_WhileLoop". (* immediate from the IH *)
+    apply IHceval2. reflexivity.  Qed.
+
+
 
 Theorem WHILE_true: forall b c,
      bequiv b BTrue  ->
@@ -12,6 +33,15 @@ Theorem WHILE_true: forall b c,
        (WHILE b DO c END)
        (WHILE BTrue DO SKIP END).
 Proof. 
-  exact GIVEUP.
+  
+intros b c st st' Hb.
+  split; intros.
+  inversion H; subst.
+  apply WHILE_true_nonterm in H. inversion H.
+  apply st.
+  apply WHILE_true_nonterm in H. inversion H.
+  apply st.
+  apply WHILE_true_nonterm in H. inversion H.
+  unfold bequiv. reflexivity.
 Qed.
 
