assignments/08/P10.v
@@ -6,6 +6,18 @@ Require Export D.
 Theorem seq_assoc : forall c1 c2 c3,
   cequiv ((c1;;c2);;c3) (c1;;(c2;;c3)).
 Proof.
-  exact GIVEUP.
+      intros. intros st st'.
+  split; intros.
+  inversion H; subst.
+  inversion H2; subst.
+  apply E_Seq with (st' := st'1). assumption.
+  apply E_Seq with (st' := st'0). assumption.
+  assumption.
+
+  inversion H; subst.
+  inversion H5; subst.
+  apply E_Seq with (st' := st'1).
+  apply E_Seq with (st' := st'0).
+  assumption.  assumption. assumption.
 Qed.
 
