assignments/08/P11.v
@@ -1,12 +1,34 @@
 Require Export D.
 
-
+Theorem update_same : forall n1 x1 x2 (st : state),
+  st x1 = n1 ->
+  (update st x1 n1) x2 = st x2.
+Proof.
+  intros. unfold update. destruct (eq_id_dec x1 x2). subst. reflexivity.
+  reflexivity.
+  Qed.
 
 (** **** Exercise: 2 stars (assign_aequiv)  *)
 Theorem assign_aequiv : forall X e,
   aequiv (AId X) e -> 
   cequiv SKIP (X ::= e).
 Proof.
-  exact GIVEUP.
+      intros. unfold aequiv in H.
+  split; intros. 
+  inversion H0; subst. 
+  
+  
+  assert (st' = (update st' X (st' X))).
+  apply functional_extensionality. intros. rewrite update_same; reflexivity. 
+
+   
+  rewrite H1 at 2. constructor. rewrite <- H. simpl. reflexivity. 
+  inversion H0; subst.
+  assert (st = update st X (aeval st e)).
+  rewrite <- H. 
+  apply functional_extensionality. intros. rewrite update_same. reflexivity.
+  simpl. reflexivity.
+  rewrite <- H1. constructor.    
+
 Qed.
 
