assignments/08/P12.v
@@ -7,6 +7,12 @@ Theorem CSeq_congruence : forall c1 c1' c2 c2',
   cequiv c1 c1' -> cequiv c2 c2' ->
   cequiv (c1;;c2) (c1';;c2').
 Proof. 
-  exact GIVEUP.
+    unfold cequiv.
+  intros. split; intros.
+  inversion H1; subst.
+  apply E_Seq with (st' := st'0). apply H.  assumption.  apply H0. assumption. 
+  inversion H1; subst.
+  apply E_Seq with (st' := st'0).
+  apply H. assumption. apply H0; assumption. 
 Qed.
 
