assignments/08/P13.v
@@ -7,6 +7,18 @@ Theorem CIf_congruence : forall b b' c1 c1' c2 c2',
   bequiv b b' -> cequiv c1 c1' -> cequiv c2 c2' ->
   cequiv (IFB b THEN c1 ELSE c2 FI) (IFB b' THEN c1' ELSE c2' FI).
 Proof.
-  exact GIVEUP.
+    unfold bequiv, cequiv.
+  intros.
+  split; intros.
+  inversion H2; subst.
+  apply E_IfTrue. rewrite <- H. assumption.
+  rewrite <- H0. assumption.
+  apply E_IfFalse. rewrite <- H. assumption.
+  rewrite <- H1. assumption.
+  inversion H2; subst.
+  apply E_IfTrue. rewrite H; assumption. 
+  rewrite H0; assumption. 
+  apply E_IfFalse. rewrite H; assumption.
+  rewrite H1; assumption.
 Qed.
 
